Added bir programs step to computeLib
Translation and step

examples/compute/src/shared/bir_computeLib.sig
@@ -6,4 +6,8 @@ sig
   val compute_exp_cv : thm -> term -> thm ;
   val translate_exp_cv : thm -> unit ;
 
+  val compute_step_EVAL : term -> term -> thm ;
+  val translate_program_cv : thm -> unit ;
+  val compute_step_cv :  thm -> term -> thm ;
+
 end
